\begin{enumerate}
	\item Let $x, y \in V , \ \ c \in F$ \\
	$\implies (aT+U)(cx+y)$ \\
	$=aT(cx+y)+U(cx+y)$ \\ 
	$=acT(x)+aT(y)+cU(x)+U(y)$\\
	$=c(aT(x)+U(x))+(aT(y)+U(y))$\\
	$=c(aT+U)(x)+(aT+U)(y)$\\
	\item $\because 1.$(If $T,U$ linear transformation $\implies aT+U$ linear transformation $\forall a \in F$) \\
	$\therefore$ The collection of all linear transformation is under addition closure and scalar multiplication closure. \\
\newpage

\begin{enumerate}
	\item[(VS1)] $\forall \ \ T,U:$ linear transformation \\$(T+U)(x) = T(x) + U(x) = U(x) = T(x) = (U+T)(x)$ \\
	$\implies T+U = U+T$\\
	\item[(VS2)] $\forall \ \ T,U,V:$ linear transformation \\
	$[(T+U)+V](x)=(T+U)(x)+V(x)=(T(x)+U(x))+V(x)$\\
	$=T(x)+(U(x)+V(x))=[T+(U+V)](x)$\\
	$\implies (T+U)+V = T+(U+V)$
	\item[(VS3)] $\exists \ \ T_0:$ linear transformation $\ni \forall \ \ T:$ linear transformation \\
	$T(x) + T_0(x) = T(x) + 0 = T(x) \implies T+T_0=T$
	\item[(VS4)] $\forall \ \ T:$ linear transformation $\exists \ \ U:$ linear transformation \\$\ni T+U = T_0$\\
	Let $U=-T$ \\
	$(T+U)(x)=(T+(-T))(x)=T(x)+(-T)(x)=T(x)-T(x)=0=T_0(x) \implies T+U=T_0$
	\item[(VS5)] $\forall \ \ T:$ linear transformation $1T(x)=T(1x)=T(x)\implies 1T=T$
	\item[(VS6)] $\forall \ \ a, b \in F $ $\forall \ \ T:$ linear transformation $(ab)T(x)=aT(bx)=a(bT(x)) \implies (ab)T=a(bT)$
	\item[(VS7)]$\forall \ \ a \in F \ \ \forall \ \ T,U$ linear transformation \\ $a(T+U)(x)=a(T(x)+U(x))$ 
	$\implies a(T+U)=aT+aU$
	\item[(VS8)]$\forall \ \ a, b \in F \ \ \forall \ \ T:$ linear transformation \\
	$(a+b)T(x) = T((a+b)x) \\ = T(ax+bx)=T(ax)+T(bx)\\=aT(x)+bT(x) \implies (a+b)T=aT+bT$
\end{enumerate}

$\implies$ The collection of all linear transformation is a vector space over $F.$




















