\begin{proof}
	Let $A,B$ and $C$ be metrics $\ni A(BC)$ is defined $\implies (AB)C$ is also defined and $A(BC) = (AB)C$
	
	Let $B \in M_{m \times n} ~ C \in M_{n \times p} \implies (BC) \in M_{m \times p} \implies A \in M_{q \times m}$
	
	$\because (AB) \in M_{q \times n}~ C \in M_{n \times p} \implies (AB)C$ is defined
	
	$\because$ By Thm 2.15.5 $\therefore L_{A(BC)} = L_AL_{BC} = L_A(L_BL_C) = (L_AL_B)L_C = L_{AB}L_C = L_{(AB)C}$
	
	$\because$ By Thm 2.15.2 $\therefore A(BC) = (AB)C$
\end{proof}
