Let $x \in V $

\begin{enumerate}
\item \(T\left(U_{1}+U_{2}\right)(x)=T\left(U_{1}(x)+U_{2}(x)\right)=T U_{2}(x)+T U_{2}(x)\)
\(\Rightarrow T\left(U_{1}+U_{2}\right)=T U_{1}+T U_{2}\)
\(\left(U_{1}+U_{2}\right) T(x)=U_{1} T(x)+U_{2} T(x)\)
\(\Rightarrow\left(U_{1}+U_{2}\right) T=U_{1} T+U_{2} T\)
\item \(T\left(U_{1} U_{2}\right)(x)=T\left(U_{1}\left(U_{2}(x)\right)\right)=\left(T U_{1}\right)\left(U_{2}(x)\right)\)
\(\Rightarrow T\left(U_{1} U_{2}\right)=\left(T U_{1}\right) U_{2}\)
\item \(T I(x)=T(x)=I T(x)\) \(\Rightarrow T I=T=I T\)
\item  \(a\left(U_{1} U_{2}\right)(x)=a\left(U_{1}\left(U_{2}(x)\right)=\left(a U_{3}\right)\left(U_{2}(x)\right)=U_{1}\left(a U_{2}(x)\right)\right.\)
\(\Rightarrow a\left(U_{1} U_{2}\right)=\left(a U_{1}\right) U_{2}=U_{1}\left(a U_{2}\right) \quad\)

\end{enumerate}
 