\begin{enumerate}
\item The $j$th column of $[L_A]_{\beta}^{\gamma} = L_A(e_j) $ $\because $\ Thm 2.13 %should be checked in our version 
	$\therefore L_A(e_j) = Ae_j$ is the $j$th column of $A \implies [L_A]_{\beta}^{\gamma} = A$
\item ($\Rightarrow$) If $L_A = L_B \implies A = [L_A]_{\beta}^{\gamma} = [L_B]_{\beta}^{\gamma} = B$ 
	
	($\Leftarrow$) If $A = B \implies L_A(x) = Ax = Bx = L_{B}(x)\implies L_{A} = L_{B}$	
\item $L_{A+B}(x) = (A + B)(x) = Ax + Bx  = L_A(x) + L_B(x)$ 

	$\implies L_{A+B} = L_A + L_B$
	
	$L_{aA}(x) = (aA)x = aAx = aL_{A}(x)\implies L_{aA} = aL_{A}\ \forall a \in F$
	

\item Let $C = [T]_{\beta}^{\gamma}$ by Thm 2.14 $[T(x)]_{\gamma} = [T]_{\beta}^{\gamma}[x]_{\beta} \Leftrightarrow T(x) = Cx = L_{C}(x)\ \forall x \in F^{n} \implies T = L_{C}$ by (2) $C$ is unique.
\item For $j = 1,\cdots ,p$ by Thm 2.13 $(AE)e_j$ is the  $j$th column of $AE$, $(AE)e_j = A(Ee_j)$ $\therefore$ $L_{AE}(e_j) = (AE)e_j = A(Ee_j) = L_A(Ee_j) = L_A(L_E(e_j)) = L_AL_Ee_j$ By cor of Thm 2.6 $\therefore L_{AE} = L_AL_E$
\item $L_{I_n}(x) = I_nx = x\ \forall x\in F^{n}$, $I_{F^{n}}(x) = x \implies L_{I_n} = I_{F^n}$ 



\end{enumerate} 