Let $\beta = \left\{v_j \ |\ 1 \leq j\leq n \right\} $ and $\gamma = \left\{ w_i\ |\ 1\leq i\leq m \right \} $ $\implies\exists ! a_{ij} , b_{ij} \in F$ for $1\leq j \leq n $ , $1\leq i \leq m$ s.t. 

\begin{enumerate}
	\item $T(v_j) = \sum_{i = 1}^m a_{ij}w_i$ and $U(v_{j}) = \sum_{i = 1}^m b_{ij} w_i $, hence 
	$$\left(T+ U \right)(v_j) = \sum_{i=1}^m(a_{ij} + b_
		{ij})wi $$
	Thus $\left([T+U]_{\beta}^{\gamma}\right)_{i j}=a_{i j}+b_{i j}=\left([T]_{\beta}^{\gamma}\right)_{i j}+\left([U]_{\beta}^{\gamma}\right)_{i j}=\left([T]_{\beta}^{\gamma}+[U]_{\beta}^{\gamma}\right)_{i j}$
$\implies [T+U]_{\beta}^{\gamma}=[T]_{\beta}^{\gamma}+[U]_{\beta}^{\gamma}$
	\item $T\left(V_{j}\right)=\sum_{i=1}^{m} a_{i j} w_{i}$ for $j=1 , \cdots n $ and $ a \in F$ then
$ a T\left(v_{j}\right) = a \sum_{i=1}^{m} a_{i j} w_{i}=\sum_{i=1}^{m} a a_{i j} w_{i} = T\left(a v_{j} \right)$
thus
$\left([a T]_{\beta}^{\gamma}\right)_{j j}=a a_{i j}=\left(a[T]_{\beta}^{\gamma}\right)_{i j}$
$\implies [a T]_{\beta}^{\gamma} = a[T]_{\beta}^{\gamma}$

\end{enumerate} 