\begin{proof}
	Let $\beta$ be a basis of $v$. Suppose $v=a_1u_1+...+a_nu_n=b_1u_1+...+b_nu_n$. We have $0=(a_1-b_1)u_1+...+(a_n-b_n)u_n$. Since $\beta$ is linear independent, we have $(a_1-b_1)=...=(a_n-b_n)$, hence $a_1=b_1,...,a_n=b_n$, which means $v$ is uniquely expressed as a linear combination of $\beta$. Conversely, suppose $v$ can be uniquely expressed as a linear combination of $\beta$. Clearly, $\beta$ generates $V$ and the representation of $0$ is unique. So if $0=a_1u_1+...+a_nu_n$, we have $a_1=...=a_n$. Thus $\beta$ is linear independent and is a basis of $V$.
\end{proof}