Let $A,B$ be two nonempty sets of $\R$

\begin{enumerate}
	\item If $A \subseteq B$, then $\sup A \leq \sup B$ and $\inf A \geq \inf B$.
	\item Show that $\inf A \leq \sup A$.
	\item Show that $\inf (-A) = -\sup A$ and $\sup (-A) = -\inf (A)$, where $-A = \{-a ~|~ a \in A\}$
	\item Show that $\sup (A+B) = \sup A + \sup B$ and $\inf (A+B) = \inf A + \inf B$, where $A + B = \{a + b ~|~ a \in A,b \in B\}$, the Minkowski sum of $A$ and $B$.
	\item If $A,B$ be two sets of positive numbers which is bounded above. Let $\alpha = \sup A,~b = \sup B$ and $C = \{ab ~|~ a \in A ,~b \in B\}$. Prove that $\sup C = ab$.
\end{enumerate}

\begin{tcolorbox}
	\begin{solution}$ $
		\begin{enumerate}[wide]
			\item Suppose $A \subseteq B$. To prove $\sup A \leq \sup B$
			\begin{enumerate}[label = $(*)$]
				\item If $A$ is unbdd above, then $B$ is also. Thus, $\sup A = + \infty = \sup B$
				\item If $A$ is bdd above then we have two cases
					\begin{enumerate}
						\item[($*_1$)] If $B$ is unbdd above, then the result follows trivilly
						\item[($*_2$)] If $B$ is bdd above, then $\sup A,~\sup B$ exist and finite, say $\sup A = \alpha$ and $\sup B = \beta$.
						
						Now, to prove that $\alpha \leq \beta$. Given $\epsilon > 0$, since $\sup A = \alpha,~\exists a \in A \ni \alpha - \epsilon < a$. Since $A \subseteq B$ and $\beta = \sup B, a \in B$ and $a \leq \beta$
					\end{enumerate}
			\end{enumerate}
			\item 
			\item 
			\item To prove $\sup (A+B) = \alpha + \beta$ If $A$ or $B$ is unbdd above, then the result follows trivially
			
			If $A$ and $B$ are bdd above,say $\sup A = \alpha$ and $\sup B = \beta$
			
			Claim: $\sup (A+B) = \alpha + \beta$
			\begin{enumerate}
				\item Given $x \in A + B, x = a+b$ for some $a \in A$ and $b \in B$. Since $\alpha = \sup A$ and $\beta = \sup B,~ a \leq \alpha $ and $b \leq \beta \implies x = a+b \leq \alpha + \beta$
				\item Given $\epsilon > 0$, since $\alpha = \sup A$ and $\beta = \sup B, \exists a \in A,b \in B,~ \alpha - \dfrac{\epsilon}{2} < a$ and $\beta - \dfrac{\epsilon}{2} < b \implies \alpha + \beta - \epsilon < a+b$ and $a + b \in A + B$
 			\end{enumerate}
 			Hence $\sup (A+B) = \alpha + \beta$
			\item
		\end{enumerate}
	\end{solution}
\end{tcolorbox}