Show that:

\begin{enumerate}
	\item $\left( \bigcup_{\alpha \in I}E_{\alpha} \right)^c = \bigcap_{a \in I}\left( E_{\alpha}\right)^c $
	\item $\left( \bigcap_{\alpha \in I} E_{\alpha}\right)^c = \bigcup_{\alpha \in I} \left( E_{\alpha} \right)^c$
\end{enumerate}

It is called De Morgan's laws.


\begin{tcolorbox}
	\begin{solution}$ $
	\begin{enumerate}
		\item 
		\begin{enumerate}
			\item[($\subseteq$)]
				let $p \in \left( \bigcup_{\alpha \in I}E_{\alpha} \right)^c \implies p \notin \bigcup_{\alpha \in I}E_{\alpha} $
				
				$\implies p \notin E_{\alpha} ~\forall \alpha \in I \implies p \in (E_{\alpha})^c~\forall \alpha \in I$
				
				$\implies p \in \bigcap_{\alpha \in I}(E_{\alpha})^c$
			\item[($\supseteq$)]
			
			let $p \in \bigcap_{\alpha \in I}(E_\alpha)^c \implies p \in (E_\alpha)^c$
			
			$\implies p \in (E_{\alpha})^c \alpha \in I \implies p \notin E_{\alpha} ~\forall \alpha \in I$
			
			$\implies p \notin \bigcup_{\alpha \in I}E_{\alpha} \implies p \in \left( \bigcup_{\alpha \in I} E_{\alpha} \right)^c$
		\end{enumerate}
		\item 
		\begin{enumerate}
			\item[($\subseteq$)]
			
			let $p \in \left( \bigcap_{\alpha \in I} E_{\alpha}\right)^c \implies p \notin \bigcap_{\alpha \in I}E_{\alpha}$
			
			$\implies p \in (E_{\alpha})^c$ for some $\alpha \in I \implies p \in \bigcup_{\alpha \in I}(E_{\alpha})^c$
			\item[($\supseteq$)]
			
			let $p \in \bigcup_{\alpha \in I}(E_{\alpha})^c \implies p \in (E_{\alpha})^c$ for some $\alpha \in I$
			
			$\implies p \notin E_{\alpha}$ for some $\alpha \in I \implies p \notin \bigcap_{\alpha \in I}E_{\alpha}$
			
			$\implies p \in \left( \bigcap_{\alpha \in I}E_{\alpha} \right)^c$
		\end{enumerate}
	\end{enumerate}
	\end{solution}
\end{tcolorbox}
