\input{settings}


\begin{document}

\section*{Midterm Answer}

\begin{enumerate}
	\item (a)(b)(d)
	\item proof:
	$(\Rightarrow)$ let $n = 2k+1, k \in \Z$
	
	$n^2 = (2k+1)^2 = 4k^2 + 4k + 1 = 4(k^2 + k) + 1$ is odd
	
	$(\Leftarrow)$ We have that $n^2$ is odd
	
	Claim: $n$ is odd
	
	Suppose not, $n = 2k, k\in \Z$ is even
	
	$n^2 = 4k^2 \rightarrow\leftarrow$ to $n^2$ is odd
	
	Hence, $n$ is odd.
	
	\item (b) $\because \forall x \exists y = x + 1$ such that $x < 2y$
	
	\item $(\exists x)(\forall y)(x \geq 2y)$
	
	\item (a) $1 \neq 3$ and $f(1) = f(3)$
	
	\item $ $
	
	P: Tom finishes his work
	
	Q: Tom can go home tonight
	
	\begin{tabular}{|c|c|c|c|c|}
	\hline
	$P$&$Q$&$\sim P$&$\sim Q$&$\sim P \rightarrow \sim Q$\\
	\hline
	T & T & F & F & T \\
	\hline
	T & F & F & T & T \\
	\hline
	F & T & T & F & F \\
	\hline
	F & F & T & T & T \\
	\hline
	\end{tabular}
	
	\item (b)(d)
	\item (1)$\{2,3,4,5\}$ (2)$\{1,2,3,4,5,6,7\}$ (3)$\{1\}$
	\item (c)(d)(f)(g)(i)(j)
	\item (a) $\{3\}$ (b) $\{\frac{3}{2},3\}$ (c) $\{\pm \sqrt{2},\frac{3}{2},3\}$ (d) $\{\pm i,\pm \sqrt{2},\frac{3}{2},3\}$
	\item (b)
	
	\newpage	
	
	\item 
	
	$(\subseteq)$ Given $x \in (A \cup B) - (A \cap B)$
	
	$\Rightarrow x \in A$ or $B$ but $x \notin A \cap B$
	
	$\Rightarrow$ If $x \in A$, but $x \notin A \cap B \Rightarrow x \in A $ but $ x \notin B \Rightarrow x \in A -B$
	If $x \in B$, but $x \notin A \cap B \Rightarrow x \in B$ but $x \notin A \Rightarrow x \in B - A$
	
	$\Rightarrow x \in (A - B) \cup (B - A)$
	
	$(\supseteq)$ Given $x \in (A - B) \cup (B - A)$
	
	$\Rightarrow$ If $x \in A$, but $x \notin B$
	
	$x \in A \Rightarrow x \in A \cup B$ and $x \notin B \Rightarrow x \notin A \cap B$
	
	$x \in (A \cup B) - (A \cap B)$
	
	If $x \in B$ but $x \notin A$
	
	$x \in B \Rightarrow x \in A \cup B$ and $x \notin A \Rightarrow x \notin A \cap B$
	
	$x \in (A \cup B) - (A \cap B)$
	
	\item Converse: If $2 < 5$, then $\sqrt{2} < \sqrt{5}$
	
	Contrapositive: If $2 \geq 5$, then $\sqrt{2} \geq \sqrt{5}$
	
	\item (a)(b)(c)
	\item True, Given $x \in A \cap C \Rightarrow x \in A$ and $x \in C$,
	
	then $x \in A \subseteq B \Rightarrow x \in B$ and $x \in C \subseteq D \Rightarrow x \in D$
	
	$\therefore	 x \in B \cap D$ Hence $A \cap C \subseteq B \cap D$


\end{enumerate}






\end{document}