\input{../settings}

\usepackage[a4paper,margin=1in]{geometry}

\begin{document}

\title{Some Result}
\author{KANG,WEI-HSIANG}
\date{}

\maketitle

\subsection*{1. When n=1}$ $

$f_1(p) = (1-p)^9 + 3p(1-p)^8$

$g_1(p) = 2p(1-p)^8 + 2p^2(1-p)^7$

$h_1(p) = 3p^2(1-p)^7$

$t_1(p) = 2p^3(1-p)^6$

\textbf{Ratios}

$\alpha_1(p)=\frac{g_1(p)}{f_1(p)} = \frac{2pq + 2p^2}{q^2+3pq} = \frac{2p}{q(1+2p)} = \frac{2p}{(1-p)(1+2p)}$

$\beta_1(p)=\frac{h_1(p)}{g_1(p)}=\frac{3p}{2q+2p}=\frac{3p}{2}$

$\gamma_1(p)=\frac{t_1(p)}{h_1(p)}=\frac{2p}{3q}$

Note: $q = (1-p)$

\textbf{Difference}

$\tilde{\epsilon_1}(p) = \alpha_1(p)-\beta_1(p)=\frac{2p}{q(1+2p)}-\frac{3p}{2} 
= \frac{4p}{2q(1+2p)} - \frac{3pq(1+2p)}{2q(1+2p)} = \frac{p}{q}(\frac{4-3q-6pq}{2+4p})
= \frac{p}{q}(\frac{6p^2-3p+1}{2+4p})$

$\tilde{\epsilon'_1}(p) = \beta_1(p) - \gamma_1(p) = \frac{3p}{2} - \frac{2p}{3q}
= \frac{9pq - 4p}{6q} = \frac{p}{q}\frac{9q-4}{6}=\frac{p}{q}\frac{5-9p}{6}$


$\tilde{\epsilon_1}(p) + \tilde{\epsilon'_1}(p) = \alpha_1(p)-\gamma_1(p) = \frac{2p}{q(1+2p)} - \frac{2p}{3q} 
= \frac{6p - 2p(1+2p)}{3q(1+2p)} = \frac{6p - 2p - 4p^2}{3q(1+2p)} = \frac{p}{q}\frac{4q}{3(1+2p)}$

Define $c_p = \frac{q}{p}$

$\epsilon_1 = c_p(\alpha_1(p) - \beta_1(p)) = \frac{6p^2 - 3p + 1}{2 + 4p}$

$\epsilon_1' = c_p(\beta_1(p) - \gamma_1(p)) = \frac{5-9p}{6}$

$\epsilon_1(p) + \epsilon_1'(p) = c_p(\alpha_1(p) - \gamma_1(p)) = \frac{4q}{3(1+2p)}$

\subsection*{2. Iterated}$ $

In this section, we shorten the notation of $(p)$, like $f_k(p)$ denote $f_k$

$f_{k+1} = f_k^3 + 6_k^2g_k + 3f_k^2h_k + 9f_kg_k^2 + 6f_kg_kh_k + 2g_k^3$

$g_{k+1} = f_k^2g_k + 4f_kg_k^2 + 2f_k^2h_k + f_k^2t_k + 8f_kg_kh_k + 3g_k^3 + 2f_kg_kt_k + 2f_kh_k^2 + 4g_k^2h_k$

$h_{k+1} = f_kg_k^2 + 4f_kg_kh_k + 2g_k^3 + 2f_kg_kt_k + 7g_k^2h_k + 3f_kh_k^2 + 2g_k^2t_k + 4g_kh_k^2 + 2f_kh_kt_k$

$t_{k+1} = g_k^3 + 6g_k^2h_k + 3g_k^2t_k + 9g_kh_k^2 + 6g_kh_kt_k + 2h_k^3$

\textbf{Ratios}

$\alpha_{n+1} = \alpha_n\frac{B_n}{A_n}$, $\beta_{n+1} = \alpha_n\frac{C_n}{B_n}$, $\gamma_{n+1} = \alpha_n\frac{D_n}{C_n}$

$A_n = 1 + 6\alpha_n + 3\alpha_n\beta_n + 9\alpha_n^2 + 6\alpha_n^2\beta_n + 2\alpha_n^3$

$B_n = 1 + 4\alpha_n + 2\beta_n + \beta_n\gamma_n + 8\alpha_n\beta_n + 3\alpha_n^2 + 2\alpha_n\beta_n\gamma_n + 2\alpha_n\beta_n^2 + 4\alpha_n^2\beta_n$

$C_n = 1 + 2\alpha_n + 4\beta_n + 2\beta_n\gamma_n + 7\alpha_n\beta_n + 3\beta_n^2 + 2\alpha_n\beta_n\gamma_n + 4\alpha_n\beta_n^2 + 2\beta_n^2\gamma_n$


$D_n = 1 + 6\beta_n + 3\beta_n\gamma_n + 9\beta_n^2 + 6\beta_n\gamma_n + 2\beta_n^3$

\newpage

\textbf{Difference}

\begin{align*}
\tilde{\epsilon}_{n+1} &= \alpha_{n+1} - \beta_{n+1} = \alpha_n\left( \frac{B_n}{A_n} - \frac{C_n}{B_n} \right) = \frac{\alpha_n}{A_nB_n}\left( B_n^2 - A_nC_n \right)\\
&= \frac{1}{A_nB_n}\left[ 
\begin{array}{l}
\tilde{\epsilon}_n^2
(4\alpha_n^3\beta_n^2 + 10\alpha_n^3\beta_n + 2\alpha^2\beta^2 + 5\alpha^3
+ 7\alpha_n^2\beta_n + \alpha_n\beta_n^2 + 4\alpha_n^2 + 2\alpha_n\beta_n + \alpha_n)+\\
\tilde{\epsilon}_n\tilde{\epsilon}_n'
(4\alpha_n^4\beta_n + 4\alpha_n^3\beta_n^2 + 10\alpha_n^3\beta_n + 6\alpha_n^2\beta_n^2+
8\alpha_n^2\beta_n + 2\alpha_n\beta_n^2 + 2\alpha_n\beta_n)+\\
\tilde{\epsilon}_n'^2
(4\alpha_n^3\beta_n^2 + 4\alpha_n^2\beta_n^2 + \alpha_n\beta_n^2)
\end{array}\right]
\end{align*}

\begin{align*}
\tilde{\epsilon'}_{n+1} &= \beta_{n+1} - \gamma_{n+1} = \alpha_n\left( \frac{C_n}{B_n} - \frac{D_n}{C_n} \right) = \alpha_n\left( \frac{C_n^2 - B_nD_n}{B_nC_n} \right)\\
&= \frac{1}{B_nC_n}\left[
\begin{array}{l}
\tilde{\epsilon}_n^2
(4\alpha_n\beta_n^4 + 12\alpha_n\beta_n^3 + 13\alpha_n\beta_n^2 + 
6\alpha_n\beta_n + \alpha_n)+\\
\tilde{\epsilon}_n\tilde{\epsilon}_n'
(4\alpha_n^2\beta_n^3 - 4\alpha_n^2\beta_n^2\gamma_n - 8\alpha_n\beta_n^4 + 
18\alpha_n\gamma_n^3 + 2\alpha_n^2\beta_n^2 + 9\alpha_n\beta_n^2 +
\alpha_n^2\beta_n + 2\alpha_n\beta_n)+\\
\tilde{\epsilon}_n'^2
(4\alpha_n\beta_n^4 + 2\alpha_n\beta_n^3 + 2\alpha_n^2\beta_n^2 + \alpha_n\beta_n^2)
\end{array}\right]
\end{align*}

\begin{align*}
\tilde{\epsilon}_{n+1} + \tilde{\epsilon}_{n+1}' &= \alpha_{n+1} - \gamma_{n+1} = 
\alpha_{n}\left( \frac{B_n}{A_n} - \frac{D_n}{C_n} \right) = 
\alpha_n\left( \frac{B_nC_n - A_nD_n}{A_nC_n} \right)\\
&= \frac{\alpha_n}{A_nC_n}(2\alpha_n + 1)(\alpha_n^2 + 3\alpha_n\beta_n + 4\alpha_n + 1)\\
&\quad (4\alpha_n\beta_n^2 + 2\alpha_n\beta_n\gamma_n - 2\beta_n^3 - 4\beta_n^2\gamma_n + 7\alpha_n\beta_n - 6\beta_n^2 - \beta_n\gamma_n + 2\alpha_n - 2\beta_n)\\
&= \frac{\alpha_n}{A_nC_n}(2\alpha_n + 1)(\alpha_n^2 + 3\alpha_n\beta_n + 4\alpha_n + 1)\\
&\quad [2\beta_n^2\tilde{\epsilon}_n + 2\beta_n^2(\tilde{\epsilon}_n+\tilde{\epsilon}_n') + 2\beta_n\gamma_n\tilde{\epsilon}_n +
6\beta_n\tilde{\epsilon}_n + \beta_n(\tilde{\epsilon}_n + \tilde{\epsilon}_n') + 2\tilde{\epsilon}_n] \hspace{10cm} \\
&= \frac{\alpha_n}{A_nC_n}(2\alpha_n + 1)(\alpha_n^2 + 3\alpha_n\beta_n + 4\alpha_n + 1)\\
&\quad [\tilde{\epsilon}_n(2\beta_n^2 + 2\beta_n\gamma_n + 6\beta_n + 2)+(\tilde{\epsilon}_n+\tilde{\epsilon'}_n)(2\beta_n^2 + \beta_n)]
\end{align*}

\newpage

\begin{align*}
A_nB_n =& 8 \alpha_n^{5} \beta_n + 28 \alpha_n^{4} \beta_n^{2} + 4 \alpha_n^{4} \beta_n \gamma_n + 12 \alpha_n^{3} \beta_n^{3} + 12 \alpha_n^{3} \beta_n^{2} \gamma_n \\
 &+ 6 \alpha_n^{5} + 70 \alpha_n^{4} \beta_n + 78 \alpha_n^{3} \beta_n^{2} + 20 \alpha_n^{3} \beta_n \gamma_n + 6 \alpha_n^{2} \beta_n^{3} + 12 \alpha_n^{2} \beta_n^{2} \gamma_n \\
 &+ 35 \alpha_n^{4} + 133 \alpha_n^{3} \beta_n + 48 \alpha_n^{2} \beta_n^{2} + 21 \alpha_n^{2} \beta_n \gamma_n + 3 \alpha_n \beta_n^{2} \gamma_n \\
 &+ 56 \alpha_n^{3} + 88 \alpha_n^{2} \beta_n + 8 \alpha_n \beta_n^{2} + 8 \alpha_n \beta_n \gamma_n + 36 \alpha_n^{2} + 23 \alpha_n \beta_n + \beta_n \gamma_n + 10 \alpha_n + 2 \beta_n + 1 
\end{align*}

\begin{align*}
B_nC_n =& 16 \alpha_n^{3} \beta_n^{3} + 8 \alpha_n^{3} \beta_n^{2} \gamma_n + 8 \alpha_n^{2} \beta_n^{4} \\
&+ 20 \alpha_n^{2} \beta_n^{3} \gamma_n + 4 \alpha_n^{2} \beta_n^{2} \gamma_n^{2} + 4 \alpha_n \beta_n^{4} \gamma_n + 4 \alpha_n \beta_n^{3} \gamma_n^{2} + 40 \alpha_n^{3} \beta_n^{2} + 6 \alpha_n^{3} \beta_n \gamma_n + 58 \alpha_n^{2} \beta_n^{3} + 44 \alpha_n^{2} \beta_n^{2} \gamma_n\\
&+ 6 \alpha_n \beta_n^{4} + 30 \alpha_n \beta_n^{3} \gamma_n + 6 \alpha_n \beta_n^{2} \gamma_n^{2} + 2 \beta_n^{3} \gamma_n^{2} \\
&+ 29 \alpha_n^{3} \beta_n + 101 \alpha_n^{2} \beta_n^{2} + 18 \alpha_n^{2} \beta_n \gamma_n + 40 \alpha_n \beta_n^{3} \\
&+ 43 \alpha_n \beta_n^{2} \gamma_n + 7 \beta_n^{3} \gamma_n + 2 \beta_n^{2} \gamma_n^{2} + 6 \alpha_n^{3} + 60 \alpha_n^{2} \beta_n + 64 \alpha_n \beta_n^{2} + 14 \alpha_n \beta_n \gamma_n + 6 \beta_n^{3} + 10 \beta_n^{2} \gamma_n \\
&+ 11 \alpha_n^{2} + 35 \alpha_n \beta_n + 11 \beta_n^{2} + 3 \beta_n \gamma_n + 6 \alpha_n + 6 \beta_n + 1
\end{align*}


\begin{align*}
\epsilon_{n+1} &= c_p(\alpha_{n+1} - \beta_{n+1}) = c_p\alpha_n\left( \frac{B_n}{A_n} - \frac{C_n}{B_n} \right) = \frac{c_p\alpha_n}{A_nB_n}\left( B_n^2 - A_nC_n \right)
= c_p\tilde{\epsilon}_{n+1}\\
&= \frac{c_p}{A_nB_n}
\left[ 
\begin{array}{l}
\tilde{\epsilon}_n^2
(4\alpha_n^3\beta_n^2 + 10\alpha_n^3\beta_n + 2\alpha^2\beta^2 + 5\alpha^3
+ 7\alpha_n^2\beta_n + \alpha_n\beta_n^2 + 4\alpha_n^2 + 2\alpha_n\beta_n + \alpha_n)+\\
\tilde{\epsilon}_n\tilde{\epsilon}_n'
(4\alpha_n^4\beta_n + 4\alpha_n^3\beta_n^2 + 10\alpha_n^3\beta_n + 6\alpha_n^2\beta_n^2+
8\alpha_n^2\beta_n + 2\alpha_n\beta_n^2 + 2\alpha_n\beta_n)+\\
\tilde{\epsilon}_n'^2
(4\alpha_n^3\beta_n^2 + 4\alpha_n^2\beta_n^2 + \alpha_n\beta_n^2)
\end{array}\right]\\
&= \frac{1}{c_pA_nB_n}
\left[ 
\begin{array}{l}
\epsilon_n^2
(4\alpha_n^3\beta_n^2 + 10\alpha_n^3\beta_n + 2\alpha^2\beta^2 + 5\alpha^3
+ 7\alpha_n^2\beta_n + \alpha_n\beta_n^2 + 4\alpha_n^2 + 2\alpha_n\beta_n + \alpha_n)+\\
\epsilon_n\epsilon_n'
(4\alpha_n^4\beta_n + 4\alpha_n^3\beta_n^2 + 10\alpha_n^3\beta_n + 6\alpha_n^2\beta_n^2+
8\alpha_n^2\beta_n + 2\alpha_n\beta_n^2 + 2\alpha_n\beta_n)+\\
\epsilon_n'^2
(4\alpha_n^3\beta_n^2 + 4\alpha_n^2\beta_n^2 + \alpha_n\beta_n^2)
\end{array}\right]\\
&= \frac{1}{A_nB_n}
\left[
\begin{array}{l}
\epsilon_n 
( 4\alpha_n^4\beta_n^2 - 4\alpha_n^3\beta_n^3 + 10\alpha_n^4\beta_n - 8\alpha_n^3\beta_n^2 + 2\alpha_n^2\beta_n^3 - 4\alpha_n^2\beta_n^2\gamma_n \\
+ 5\alpha_n^4 + 2\alpha_n^3\beta_n - 6\alpha_n^2\beta_n\gamma_n - \alpha_n\beta_n^2\gamma_n + 4\alpha_n^3 - 2\alpha_n^2\beta_n - 2\alpha_n\beta_n\gamma_n + \alpha_n^2 - \alpha_n\beta_n ) + \\
\epsilon_n'
(4\alpha_n^5\beta_n - 4\alpha_n^3\beta_n^2\gamma_n + 10\alpha_n^4\beta_n - 8\alpha_n^3\beta_n^2 + 2\alpha_n^2\beta_n^3 - 4\alpha_n^2\beta_n^2\gamma_n \\
+ 2\alpha_n^3\beta_n - \alpha_n\beta_n^2\gamma_n - \alpha_n^2\beta_n^2 )
\end{array}\right]
\end{align*}

\begin{align*}
\epsilon'_{n+1} &= c_p(\beta_{n+1} - \gamma_{n+1}) = c_p\alpha_n\left( \frac{C_n}{B_n} - \frac{D_n}{C_n} \right) = c_p\alpha_n\left( \frac{C_n^2 - B_nD_n}{B_nC_n} \right)\\
&= \frac{1}{c_pB_nC_n}\left[
\begin{array}{l}
\epsilon_n^2
(4\alpha_n\beta_n^4 + 12\alpha_n\beta_n^3 + 13\alpha_n\beta_n^2 + 
6\alpha_n\beta_n + \alpha_n)+\\
\epsilon_n\epsilon_n'
(4\alpha_n^2\beta_n^3 - 4\alpha_n^2\beta_n^2\gamma_n - 8\alpha_n\beta_n^4 + 
18\alpha_n\gamma_n^3 + 2\alpha_n^2\beta_n^2 + 9\alpha_n\beta_n^2 +
\alpha_n^2\beta_n + 2\alpha_n\beta_n)+\\
\epsilon_n'^2
(4\alpha_n\beta_n^4 + 2\alpha_n\beta_n^3 + 2\alpha_n^2\beta_n^2 + \alpha_n\beta_n^2)
\end{array}\right]\\
&= \frac{1}{B_nC_n}\left[
\begin{array}{l}
\epsilon_n(4\alpha_n^2\beta_n^4 - 4\alpha_n\beta_n^3\gamma_n^2 + 14\alpha_n^2\beta_n^3 - 12\alpha_n\beta_n^3\gamma_n - 2\alpha_n^2\beta_n^2\gamma_n \\
- 12\alpha_n\beta_n^3 - \alpha_n\beta_n^2\gamma_n + 13\alpha_n^2\beta_n^2 - 2\alpha_n\beta_n\gamma_n + 6\alpha_n^2\beta_n - 4\alpha_n\beta_n^2 + \alpha_n^2 - \alpha_n\beta_n) + \\
\epsilon_n' (4\alpha_n^3\beta_n^3 - 4\alpha_n^3\beta_n^2\gamma_n + 14\alpha_n^2\beta_n^3 - 2\alpha_n\beta_n^3\gamma_n - 10\alpha_n^2\beta_n^3 \\
- 2\alpha_n^2\beta_n^2\gamma_n - 7\alpha_n\beta_n^3 - \alpha_n\beta_n^2\gamma_n + \alpha_n^3\beta_n + 7\alpha_n^2\beta_n^2)
\end{array}\right]\\
\end{align*}


\end{document}